core(OQL): WIP for OQL order by
Signed-off-by: Jerome Simeon <jeromesimeon@me.com>

compiler/core/Utils/SortableData.v
@@ -15,6 +15,7 @@
 Require Import Orders.
 Require Import Equivalence.
 Require Import EquivDec.
+Require Import Permutation.
 Require Import Compare_dec.
 Require Import Lia.
 Require Import String.
@@ -161,6 +162,13 @@ Module SortableDataOrder <: OrderedTypeFull with Definition t:=sdata.
     | Gt => False
     end.
 
+  Definition gt (a b:sdata) :=
+    match compare a b with
+    | Lt => False
+    | Eq => False
+    | Gt => True
+    end.
+
   Lemma le_lteq : forall x y : t, le x y <-> lt x y \/ eq x y.
   Proof.
     intros.
@@ -192,6 +200,28 @@ Module SortableDataOrder <: OrderedTypeFull with Definition t:=sdata.
     destruct l2.
     - apply (asymmetry H0 H1).
     - rewrite H1 in H0. apply (irreflexivity H0).
+  Qed.
+
+  Lemma le_not_gt a b :
+    le a b -> ~(gt a b).
+  Proof.
+    unfold not; intros.
+    unfold le, gt in *.
+    destruct (compare a b); simpl in *; congruence.
+  Qed.
+
+  Lemma compare_transitive x y z c:
+    compare x y = c -> compare y z = c -> compare x z = c.
+  Proof.
+    intros; destruct c.
+    - rewrite compare_eq_iff in *; subst; reflexivity.
+    - generalize (@StrictOrder_Transitive t lt lt_strorder); unfold Transitive; intros.
+      apply (H1 x y z); assumption.
+    - unfold compare in *.
+      destruct x; destruct y; destruct z; try reflexivity; try congruence.
+      + apply (Zgt_trans z0 z1 z H H0).
+      + generalize (StringOrder.gt_transitive s s0 s1); intros.
+        auto.
   Qed.
 
 End SortableDataOrder.
@@ -277,23 +307,32 @@ Module LexicographicDataOrder <: OrderedTypeFull with Definition t:=list sdata.
     destruct (SortableDataOrder.compare a s); intuition; congruence.
   Qed.
 
+  Lemma compare_transitive x y z c:
+    compare x y = c -> compare y z = c -> compare x z = c.
+  Proof.
+    revert x y z.
+    induction x; destruct y; destruct z; simpl; eauto; try congruence.
+    intros. specialize (IHx y z).
+    generalize (@StrictOrder_Transitive _ _ (SortableDataOrder.lt_strorder) a s s0).
+    unfold SortableDataOrder.lt. intros AC.
+    case_eq (SortableDataOrder.compare a s); 
+      intros re; rewrite re in *; try congruence;
+        case_eq (SortableDataOrder.compare s s0); 
+        intros re2; rewrite re2 in *; try congruence;
+          try rewrite SortableDataOrder.compare_eq_iff in *; subst;
+            try rewrite re in*; try rewrite re2 in *;
+              try rewrite AC by trivial; 
+              try rewrite SortableDataOrder.compare_refl_eq; 
+              auto.
+    rewrite (SortableDataOrder.compare_transitive _ _ _ Gt re re2).
+    reflexivity.
+  Qed.
+
   Global Instance lt_strorder : StrictOrder lt.
   Proof.
     split; repeat red; unfold lt.
     - intros a H; rewrite compare_refl_eq in H. discriminate. 
-    - induction x; destruct y; destruct z; simpl; eauto; try congruence.
-      intros. specialize (IHx y z).
-      generalize (@StrictOrder_Transitive _ _ (SortableDataOrder.lt_strorder) a s s0).
-      unfold SortableDataOrder.lt. intros AC.
-      case_eq (SortableDataOrder.compare a s); 
-        intros re; rewrite re in *; try congruence;
-          case_eq (SortableDataOrder.compare s s0); 
-          intros re2; rewrite re2 in *; try congruence;
-            try rewrite SortableDataOrder.compare_eq_iff in *; subst;
-              try rewrite re in*; try rewrite re2 in *;
-                try rewrite AC by trivial; 
-                try rewrite SortableDataOrder.compare_refl_eq; 
-                auto.
+    - intros. apply (compare_transitive x y z Lt); assumption.
   Qed.
 
   Lemma lt_compat : Proper (eq ==> eq ==> iff) lt.
@@ -376,7 +415,24 @@ Module LexicographicDataOrder <: OrderedTypeFull with Definition t:=list sdata.
     - rewrite H2; left; assumption.
     - rewrite H1 in H2; rewrite H2; right; reflexivity.
   Qed.
-  
+
+  Lemma flip_not_le l l0:
+    ~le l l0 -> le l0 l.
+  Proof.
+    intros.
+    unfold le in *.
+    unfold not in *.
+    case_eq (compare l l0); intros; rewrite H0 in H; try congruence.
+    - assert False by (apply H; trivial); contradiction.
+    - assert False by (apply H; trivial); contradiction.
+    - case_eq (compare l0 l); intros; try trivial.
+      assert (compare l l = Gt)
+        by (apply (compare_transitive l l0 l); assumption).
+      assert (compare l l = Eq).
+      rewrite compare_eq_iff; reflexivity.
+      congruence.
+  Qed.
+
 End LexicographicDataOrder.
 
 Section DictSort.
@@ -503,6 +559,53 @@ Section DictSort.
         exists (l1, d); auto.
   Qed.
 
+  Lemma flip_not_dict_field_le a a0:
+    ~dict_field_le a a0 -> dict_field_le a0 a.
+  Proof.
+    intros.
+    unfold dict_field_le in *.
+    destruct a; destruct a0; simpl in *.
+    apply LexicographicDataOrder.flip_not_le.
+    assumption.
+  Qed.
+
+  Lemma insertion_sort_insert_perm (l:list sortable_data) (a:sortable_data) :
+    Permutation (a::l) (insertion_sort_insert dict_field_le_dec a l).
+  Proof.
+    revert l.
+    induction l; simpl.
+    - repeat constructor.
+    - destruct (dict_field_le_dec a a0); trivial.
+      destruct (dict_field_le_dec a0 a); trivial.
+      + rewrite perm_swap.
+        rewrite Permutation_cons; try eassumption; trivial.
+      + apply (flip_not_dict_field_le a a0) in n.
+        contradiction.
+  Qed.
+
+  Lemma insertion_sort_on_perm_insert_perm (l l':list sortable_data) (a:sortable_data) :
+    Permutation l l' ->
+    Permutation (a::l) (insertion_sort_insert dict_field_le_dec a l').
+  Proof.
+    intros.
+    assert (Permutation (a :: l') (a :: l))
+      by (apply Permutation_sym; apply perm_skip; assumption).
+    apply Permutation_sym in H0.
+    generalize (insertion_sort_insert_perm l' a); intros.
+    apply (Permutation_trans H0 H1).
+  Qed.
+
+  Lemma dict_sort_permutation l :
+    Permutation (dict_sort l) l.
+  Proof.
+    revert l.
+    induction l; simpl in *.
+    - constructor.
+    - apply Permutation_sym.
+      apply insertion_sort_on_perm_insert_perm.
+      apply Permutation_sym; assumption.
+  Qed.
+
 End DictSort.
 
 Section SortByGen.
@@ -525,7 +628,15 @@ Section SortByGen.
          (lift sort_sortable_coll
                (fsortable_coll_of_coll scl coll)).
 
-  Lemma sort_sortable_coll_sorted {A:Set} (scl:list (A -> option sdata)) (l1: list A)
+  Lemma sort_sortable_coll_sorted {A:Set} (l: @sortable_coll A):
+    is_list_sorted dict_field_le_dec (sort_sortable_coll l) = true.
+  Proof.
+    intros.
+    unfold sort_sortable_coll.
+    apply dict_sort_sorted.
+  Qed.
+
+  Lemma lift_sort_sortable_coll_sorted {A:Set} (scl:list (A -> option sdata)) (l1: list A)
     (l2: sortable_coll):
     lift sort_sortable_coll (fsortable_coll_of_coll scl l1) = Some l2 ->
     is_list_sorted dict_field_le_dec l2 = true.
@@ -535,19 +646,78 @@ Section SortByGen.
     case_eq (fsortable_coll_of_coll scl l1); intros; rewrite H0 in H; simpl;
       [|congruence].
     inversion H; subst; clear H.
-    unfold sort_sortable_coll.
-    apply dict_sort_sorted.
+    apply sort_sortable_coll_sorted.
   Qed.
 
-  Lemma sort_sortable_coll_StronglySorted {A:Set} (scl:list (A -> option sdata)) (l1: list A)
-    (l2: sortable_coll):
+  Lemma sort_sortable_coll_StronglySorted {A:Set} (l: @sortable_coll A):
+    StronglySorted dict_field_le (sort_sortable_coll l).
+  Proof.
+    rewrite <- is_list_sorted_StronglySorted.
+    apply sort_sortable_coll_sorted.
+    unfold Transitive; apply dict_field_le_transitive.
+  Qed.
+
+  Lemma lift_sort_sortable_coll_StronglySorted {A:Set} (scl:list (A -> option sdata))
+        (l1: list A)
+        (l2: sortable_coll) :
     lift sort_sortable_coll (fsortable_coll_of_coll scl l1) = Some l2 ->
     StronglySorted dict_field_le l2.
   Proof.
     intros.
     rewrite <- is_list_sorted_StronglySorted.
-    eapply sort_sortable_coll_sorted; apply H.
+    eapply lift_sort_sortable_coll_sorted; apply H.
     unfold Transitive; apply dict_field_le_transitive.
   Qed.
 
+  Lemma fsortable_data_of_data_snd {A:Set} (scl:list (A -> option sdata)) a s :
+    fsortable_data_of_data a scl = Some s ->
+    a = snd s.
+  Proof.
+    intros.
+    destruct s; simpl in *.
+    unfold fsortable_data_of_data in H.
+    unfold fget_criterias in H.
+    unfold lift in H.
+    destruct (lift_map (fun f : A -> option sdata => f a) scl); simpl in H;
+      [|congruence].
+    inversion H; subst.
+    reflexivity.
+  Qed.
+
+  Lemma lift_map_sortable_data_perm {A:Set} (scl:list (A -> option sdata)) l l':
+    lift_map (fun d : A => fsortable_data_of_data d scl) l = Some l' ->
+    Permutation (map snd l') l.
+  Proof.
+    intros.
+    revert l' H.
+    induction l; intros; simpl in *.
+    - inversion H; constructor.
+    - case_eq (fsortable_data_of_data a scl);
+        intros; rewrite H0 in H; simpl in *; try congruence.
+      unfold lift in H.
+      case_eq (lift_map (fun d : A => fsortable_data_of_data d scl) l);
+        intros; rewrite H1 in H; simpl in *; try congruence.
+      inversion H; simpl.
+      assert (a = snd s) by apply (fsortable_data_of_data_snd scl a s H0).
+      subst.
+      apply perm_skip.
+      apply IHl.
+      assumption.
+  Qed.
+
+  Lemma sort_sortable_coll_permuation {A:Set} (scl:list (A -> option sdata)) l l1 :
+    fsortable_coll_of_coll scl l1 = Some l ->
+    Permutation l1 (coll_of_sortable_coll (sort_sortable_coll l)).
+  Proof.
+    intros.
+    unfold sort_sortable_coll.
+    unfold fsortable_coll_of_coll in H.
+    unfold coll_of_sortable_coll.
+    assert (Permutation (map snd l) l1)
+      by (apply (lift_map_sortable_data_perm scl); assumption).
+    apply (Permutation_trans (l':= (map snd l))).
+    - apply Permutation_sym; assumption.
+    - apply Permutation_map. apply Permutation_sym. apply dict_sort_permutation.
+  Qed.
+  
 End SortByGen.
